⊢ incomparable_re_sets

src/friedberg_muchnik.lean
@@ -1,24 +1,71 @@
-import its reducibility
+import its reducibility its_computable
 
 open encodable denumerable
 
 attribute [simp] set.set_of_app_iff
 
 namespace friedberg_muchnik
-
+open rcomputable rcomputable₂
 def str : strategy 1 := default _
 
 def generator : ℕ → (Tree 0 × (list ℕ × list ℕ))
 | 0       := ([], [], [])
 | (s + 1) :=
     let μ  : Tree 0 := (generator s).1, 
-        I₀ : list ℕ := (generator s).2.1,
-        I₁ : list ℕ := (generator s).2.2,
+        L₀ : list ℕ := (generator s).2.1,
+        L₁ : list ℕ := (generator s).2.2,
         η  : Tree 1 := up[str] μ in
     match η.length.bodd with
-    | ff := if ⟦η.length.div2⟧ᵪ^I₀.chr [(λ[str] μ).weight] η.weight = some ff then (∞ :: μ, I₀, η.weight :: I₁) else (𝟘 :: μ, I₀, I₁)
-    | tt := if ⟦η.length.div2⟧ᵪ^I₁.chr [(λ[str] μ).weight] η.weight = some ff then (∞ :: μ, η.weight :: I₀, I₁) else (𝟘 :: μ, I₀, I₁)
+    | ff := if ⟦η.length.div2⟧ᵪ^L₀.chr [(λ[str] μ).weight] η.weight = some ff then (∞ :: μ, L₀, η.weight :: L₁)
+            else (𝟘 :: μ, L₀, L₁)
+    | tt := if ⟦η.length.div2⟧ᵪ^L₁.chr [(λ[str] μ).weight] η.weight = some ff then (∞ :: μ, η.weight :: L₀, L₁)
+            else (𝟘 :: μ, L₀, L₁)
     end
+
+lemma computable.generator : computable generator :=
+begin
+  let F : ℕ → (Tree 0 × list ℕ × list ℕ) :=
+  nat.elim ([], [], []) (λ s IH,
+    let μ  : Tree 0 := IH.1, 
+        L₀ : list ℕ := IH.2.1,
+        L₁ : list ℕ := IH.2.2,
+        η  : Tree 1 := up[str] μ in
+    cond η.length.bodd
+      (if ⟦η.length.div2⟧ᵪ^L₁.chr [(λ[str] μ).weight] η.weight = some ff then (∞ :: μ, η.weight :: L₀, L₁)
+       else (𝟘 :: μ, L₀, L₁))
+      (if ⟦η.length.div2⟧ᵪ^L₀.chr [(λ[str] μ).weight] η.weight = some ff then (∞ :: μ, L₀, η.weight :: L₁)
+       else (𝟘 :: μ, L₀, L₁))),
+  have : computable F,
+  { refine rcomputable.computable_of_rcomp _,
+    refine nat_elim' id ((const list.nil).pair ((const list.nil).pair (const list.nil))) _,
+    refine rcomputable.cond
+      (nat_bodd.comp $ list_length.comp (strategy.rcomputable.up.comp (fst.comp snd.to_unary₂))) _ _,
+    { refine rcomputable.ite ((rcomputable₂.to_bool_eq _).comp _ (const (some ff)))
+        ((list_cons.comp (const ∞) (fst.comp snd.to_unary₂)).pair
+          ((list_cons.comp (strategy.rcomputable.Tree_weight.comp (strategy.rcomputable.up.comp (fst.comp snd.to_unary₂)))
+            (fst.comp (snd.comp snd.to_unary₂))).pair
+              (snd.comp (snd.comp snd.to_unary₂))))
+        ((list_cons.comp (const 𝟘) (fst.comp snd.to_unary₂)).pair (snd.comp snd.to_unary₂)),
+      refine rcomputable.univn_tot_s _ _
+        (nat_div2.comp (list_length.comp (strategy.rcomputable.up.comp (fst.comp snd.to_unary₂))))
+        (list_chr.comp (snd.comp (snd.comp (snd.comp snd.to_unary₁))) snd)
+        (strategy.rcomputable.Tree_weight.comp (strategy.rcomputable.lambda.comp (fst.comp snd.to_unary₂)))
+        (strategy.rcomputable.Tree_weight.comp (strategy.rcomputable.up.comp (fst.comp snd.to_unary₂))) },
+    { refine rcomputable.ite ((rcomputable₂.to_bool_eq _).comp _ (const (some ff)))
+        ((list_cons.comp (const ∞) (fst.comp snd.to_unary₂)).pair
+          ((fst.comp (snd.comp snd.to_unary₂)).pair
+            (list_cons.comp (strategy.rcomputable.Tree_weight.comp (strategy.rcomputable.up.comp (fst.comp snd.to_unary₂)))
+              (snd.comp (snd.comp snd.to_unary₂)))))
+        ((list_cons.comp (const 𝟘) (fst.comp snd.to_unary₂)).pair (snd.comp snd.to_unary₂)),
+      refine rcomputable.univn_tot_s _ _
+        (nat_div2.comp (list_length.comp (strategy.rcomputable.up.comp (fst.comp snd.to_unary₂))))
+        (list_chr.comp (fst.comp (snd.comp (snd.comp snd.to_unary₁))) snd)
+        (strategy.rcomputable.Tree_weight.comp (strategy.rcomputable.lambda.comp (fst.comp snd.to_unary₂)))
+        (strategy.rcomputable.Tree_weight.comp (strategy.rcomputable.up.comp (fst.comp snd.to_unary₂))) } },
+  exact this.of_eq (λ s, by {
+    induction s with s IH; simp[F, generator],
+    { simp[F] at IH, simp[IH], cases C : (list.length (up[str] (generator s).fst)).bodd; simp[C, generator] } })
+end
 
 def Λ : Path 0 := ⟨λ s, (generator s).fst, λ s,
   by { cases C : (up[str] (generator s).1).length.bodd; simp[generator, C],
@@ -38,91 +85,125 @@ lemma Λ_app_eq (s : ℕ) : Λ s = (generator s).1 := rfl
 
 @[simp] lemma Λ_empty : Λ 0 = [] := rfl
 
-def I₀ (s : ℕ) : list ℕ := (generator s).2.1
+def L₀ (s : ℕ) : list ℕ := (generator s).2.1
 
-@[simp] lemma I₀_empty : I₀ 0 = [] := rfl
+@[simp] lemma L₀_empty : L₀ 0 = [] := rfl
 
-def I₁ (s : ℕ) : list ℕ := (generator s).2.2
+def L₁ (s : ℕ) : list ℕ := (generator s).2.2
 
-@[simp] lemma I₁_empty : I₁ 0 = [] := rfl
+@[simp] lemma L₁_empty : L₁ 0 = [] := rfl
 
-def I₀_inf : set ℕ := {n | ∃ s, n ∈ I₀ s}
+def I₀ : set ℕ := {n | ∃ s, n ∈ L₀ s}
 
-def I₁_inf : set ℕ := {n | ∃ s, n ∈ I₁ s}
+def I₁ : set ℕ := {n | ∃ s, n ∈ L₁ s}
+
+lemma I₀_re : r.e. I₀ :=
+begin
+  suffices : 𝚺⁰1 I₀,
+  { refine sigma_pred1_iff_re.mp this },
+  let A : set ℕ := {n | n.unpair.1 ∈ (L₀ n.unpair.2)},
+  simp[sigma_pred],
+  refine ⟨A, _⟩,
+  have : computable_pred A,
+  { refine ⟨λ a, classical.dec _, _⟩,
+    have : computable (λ a : ℕ, (L₀ a.unpair.2).chr a.unpair.1),
+      from rcomputable.computable_of_rcomp (rcomputable.list_chr.comp
+      (fst.comp $ snd.comp $ computable.generator.to_rcomp.comp (snd.comp nat_unpaired))
+      (fst.comp nat_unpaired)),
+    exact this.of_eq (λ a, by simp[A, list.chr]) },
+  exact ⟨this, by { ext a, simp[I₀] }⟩
+end
+
+lemma I₁_re : r.e. I₁ :=
+begin
+  suffices : 𝚺⁰1 I₁,
+  { refine sigma_pred1_iff_re.mp this },
+  let A : set ℕ := {n | n.unpair.1 ∈ (L₁ n.unpair.2)},
+  simp[sigma_pred],
+  refine ⟨A, _⟩,
+  have : computable_pred A,
+  { refine ⟨λ a, classical.dec _, _⟩,
+    have : computable (λ a : ℕ, (L₁ a.unpair.2).chr a.unpair.1),
+      from rcomputable.computable_of_rcomp (rcomputable.list_chr.comp
+      (snd.comp $ snd.comp $ computable.generator.to_rcomp.comp (snd.comp nat_unpaired))
+      (fst.comp nat_unpaired)),
+    exact this.of_eq (λ a, by simp[A, list.chr]) },
+  exact ⟨this, by { ext a, simp[I₁] }⟩
+end
 
 @[reducible]
 def directing_sentence₀ (s : ℕ) : Prop :=
-⟦(up[str] (Λ s)).length.div2⟧ᵪ^(I₀ s).chr [(λ[str] (Λ s)).weight] (up[str] (Λ s)).weight = ff
+⟦(up[str] (Λ s)).length.div2⟧ᵪ^(L₀ s).chr [(λ[str] (Λ s)).weight] (up[str] (Λ s)).weight = ff
 
 @[reducible]
 def directing_sentence₁ (s : ℕ) : Prop :=
-⟦(up[str] (Λ s)).length.div2⟧ᵪ^(I₁ s).chr [(λ[str] (Λ s)).weight] (up[str] (Λ s)).weight = ff
+⟦(up[str] (Λ s)).length.div2⟧ᵪ^(L₁ s).chr [(λ[str] (Λ s)).weight] (up[str] (Λ s)).weight = ff
 
 lemma generator_eq_of_pi_of_even {s : ℕ} (even : (up[str] (Λ s)).length.bodd = ff) :
-  directing_sentence₀ s → generator (s + 1) = (∞ :: Λ s, I₀ s, (up[str] (Λ s)).weight :: I₁ s) := λ C,
-by { simp[directing_sentence₀, I₀, I₁, Λ_app_eq] at C even, simp[generator, even, C, Λ_app_eq, I₀, I₁] }
+  directing_sentence₀ s → generator (s + 1) = (∞ :: Λ s, L₀ s, (up[str] (Λ s)).weight :: L₁ s) := λ C,
+by { simp[directing_sentence₀, L₀, L₁, Λ_app_eq] at C even, simp[generator, even, C, Λ_app_eq, L₀, L₁] }
 
 lemma generator_eq_of_sigma_of_even {s : ℕ} (even : (up[str] (Λ s)).length.bodd = ff) :
-  ¬directing_sentence₀ s → generator (s + 1) = (𝟘 :: Λ s, I₀ s, I₁ s) := λ C,
-by { simp[directing_sentence₀, I₀, I₁, Λ_app_eq] at C even, simp[generator, even, C, Λ_app_eq, I₀, I₁], intros h, contradiction }
+  ¬directing_sentence₀ s → generator (s + 1) = (𝟘 :: Λ s, L₀ s, L₁ s) := λ C,
+by { simp[directing_sentence₀, L₀, L₁, Λ_app_eq] at C even, simp[generator, even, C, Λ_app_eq, L₀, L₁], intros h, contradiction }
 
 lemma generator_eq_of_pi_of_odd {s : ℕ} (odd : (up[str] (Λ s)).length.bodd = tt) :
-  directing_sentence₁ s → generator (s + 1) = (∞ :: Λ s, (up[str] (Λ s)).weight :: I₀ s, I₁ s) := λ C,
-by { simp[directing_sentence₁, I₀, I₁, Λ_app_eq] at C odd, simp[generator, odd, C, Λ_app_eq, I₀, I₁] }
+  directing_sentence₁ s → generator (s + 1) = (∞ :: Λ s, (up[str] (Λ s)).weight :: L₀ s, L₁ s) := λ C,
+by { simp[directing_sentence₁, L₀, L₁, Λ_app_eq] at C odd, simp[generator, odd, C, Λ_app_eq, L₀, L₁] }
 
 lemma generator_eq_of_sigma_of_odd {s : ℕ} (odd : (up[str] (Λ s)).length.bodd = tt) :
-  ¬directing_sentence₁ s → generator (s + 1) = (𝟘 :: Λ s, I₀ s, I₁ s) := λ C,
-by { simp[directing_sentence₁, I₀, I₁, Λ_app_eq] at C odd, simp[generator, odd, C, Λ_app_eq, I₀, I₁], intros h, contradiction }
+  ¬directing_sentence₁ s → generator (s + 1) = (𝟘 :: Λ s, L₀ s, L₁ s) := λ C,
+by { simp[directing_sentence₁, L₀, L₁, Λ_app_eq] at C odd, simp[generator, odd, C, Λ_app_eq, L₀, L₁], intros h, contradiction }
 
-lemma I₁_eq_of_pi_of_even {s : ℕ} (even : (up[str] (Λ s)).length.bodd = ff) :
-  directing_sentence₀ s → I₁ (s + 1) = (up[str] (Λ s)).weight :: I₁ s := λ C,
-by simp[I₁, generator_eq_of_pi_of_even even C]
+lemma L₁_eq_of_pi_of_even {s : ℕ} (even : (up[str] (Λ s)).length.bodd = ff) :
+  directing_sentence₀ s → L₁ (s + 1) = (up[str] (Λ s)).weight :: L₁ s := λ C,
+by simp[L₁, generator_eq_of_pi_of_even even C]
 
-lemma I₁_eq_of_sigma_of_even {s : ℕ} (even : (up[str] (Λ s)).length.bodd = ff) :
-  ¬directing_sentence₀ s → I₁ (s + 1) = I₁ s := λ C,
-by simp[I₁, generator_eq_of_sigma_of_even even C]
+lemma L₁_eq_of_sigma_of_even {s : ℕ} (even : (up[str] (Λ s)).length.bodd = ff) :
+  ¬directing_sentence₀ s → L₁ (s + 1) = L₁ s := λ C,
+by simp[L₁, generator_eq_of_sigma_of_even even C]
 
-lemma I₀_eq_of_pi_of_odd {s : ℕ} (odd : (up[str] (Λ s)).length.bodd = tt) :
-  directing_sentence₁ s → I₀ (s + 1) = (up[str] (Λ s)).weight :: I₀ s := λ C,
-by simp[I₀, generator_eq_of_pi_of_odd odd C]
+lemma L₀_eq_of_pi_of_odd {s : ℕ} (odd : (up[str] (Λ s)).length.bodd = tt) :
+  directing_sentence₁ s → L₀ (s + 1) = (up[str] (Λ s)).weight :: L₀ s := λ C,
+by simp[L₀, generator_eq_of_pi_of_odd odd C]
 
-lemma I₀_eq_of_sigma_of_odd {s : ℕ} (odd : (up[str] (Λ s)).length.bodd = tt) :
-  ¬directing_sentence₁ s → I₀ (s + 1) = I₀ s := λ C,
-by simp[I₀, generator_eq_of_sigma_of_odd odd C]
+lemma L₀_eq_of_sigma_of_odd {s : ℕ} (odd : (up[str] (Λ s)).length.bodd = tt) :
+  ¬directing_sentence₁ s → L₀ (s + 1) = L₀ s := λ C,
+by simp[L₀, generator_eq_of_sigma_of_odd odd C]
 
-@[simp] lemma I₁_eq_of_odd {s : ℕ} (odd : (up[str] (Λ s)).length.bodd = tt) : I₁ (s + 1) = I₁ s :=
+@[simp] lemma L₁_eq_of_odd {s : ℕ} (odd : (up[str] (Λ s)).length.bodd = tt) : L₁ (s + 1) = L₁ s :=
 by { by_cases C : directing_sentence₁ s,
-     simp[I₁, generator_eq_of_pi_of_odd odd C], simp[I₁, generator_eq_of_sigma_of_odd odd C] }
+     simp[L₁, generator_eq_of_pi_of_odd odd C], simp[L₁, generator_eq_of_sigma_of_odd odd C] }
 
-@[simp] lemma I₀_eq_of_even {s : ℕ} (even : (up[str] (Λ s)).length.bodd = ff) : I₀ (s + 1) = I₀ s :=
+@[simp] lemma L₀_eq_of_even {s : ℕ} (even : (up[str] (Λ s)).length.bodd = ff) : L₀ (s + 1) = L₀ s :=
 by { by_cases C : directing_sentence₀ s,
-     simp[I₀, generator_eq_of_pi_of_even even C], simp[I₀, generator_eq_of_sigma_of_even even C] }
+     simp[L₀, generator_eq_of_pi_of_even even C], simp[L₀, generator_eq_of_sigma_of_even even C] }
 
-lemma mem_I₁_inf_of_pi_of_even {s} (even : (up[str] (Λ s)).length.bodd = ff) (pi : directing_sentence₀ s) :
-  (up[str] (Λ s)).weight ∈ I₁_inf := ⟨s + 1, by simp[I₁_eq_of_pi_of_even even pi]⟩
+lemma mem_I₁_of_pi_of_even {s} (even : (up[str] (Λ s)).length.bodd = ff) (pi : directing_sentence₀ s) :
+  (up[str] (Λ s)).weight ∈ I₁ := ⟨s + 1, by simp[L₁_eq_of_pi_of_even even pi]⟩
 
-lemma mem_I₀_inf_of_pi_of_odd {s} (odd : (up[str] (Λ s)).length.bodd = tt) (pi : directing_sentence₁ s) :
-  (up[str] (Λ s)).weight ∈ I₀_inf := ⟨s + 1, by simp[I₀_eq_of_pi_of_odd odd pi]⟩
+lemma mem_I₀_of_pi_of_odd {s} (odd : (up[str] (Λ s)).length.bodd = tt) (pi : directing_sentence₁ s) :
+  (up[str] (Λ s)).weight ∈ I₀ := ⟨s + 1, by simp[L₀_eq_of_pi_of_odd odd pi]⟩
 
-lemma mem_I₁_iff (t a : ℕ) :
-  a ∈ I₁ t ↔ ∃ s < t, (up[str] (Λ s)).length.bodd = ff ∧ a = (up[str] (Λ s)).weight ∧ directing_sentence₀ s :=
+lemma mem_L₁_iff (t a : ℕ) :
+  a ∈ L₁ t ↔ ∃ s < t, (up[str] (Λ s)).length.bodd = ff ∧ a = (up[str] (Λ s)).weight ∧ directing_sentence₀ s :=
 begin
   induction t with t IH,
   { simp },
   { rcases C : (up[str] (Λ t)).length.bodd with (C | C),
     { by_cases C₂ : directing_sentence₀ t,
-      { simp[I₁_eq_of_pi_of_even C C₂, IH], split,
+      { simp[L₁_eq_of_pi_of_even C C₂, IH], split,
         { rintros (rfl | ⟨s, lt, s_even, rfl, pi⟩),
           { exact ⟨t, lt_add_one t, C, rfl, C₂⟩ }, { refine ⟨s, nat.lt.step lt, s_even, rfl, pi⟩ } },
         { rintros ⟨s, lt_s, s_even, rfl, pi⟩,
           have : s < t ∨ s = t, from lt_or_eq_of_le (nat.lt_succ_iff.mp lt_s),
           rcases this with (lt | rfl), { right, refine ⟨s, lt, s_even, rfl, pi⟩ }, { left, simp } } },
-      { simp[I₁_eq_of_sigma_of_even C C₂, IH], split,
+      { simp[L₁_eq_of_sigma_of_even C C₂, IH], split,
         { rintros ⟨s, lt_s, s_even, rfl, pi⟩, refine ⟨s, nat.lt.step lt_s, s_even, rfl, pi⟩ },
         { rintros ⟨s, lt_s, s_even, rfl, pi⟩,
           have : s < t ∨ s = t, from lt_or_eq_of_le (nat.lt_succ_iff.mp lt_s),
           rcases this with (lt | rfl), { refine ⟨s, lt, s_even, rfl, pi⟩ }, { exfalso, contradiction } } } },
-    { simp[I₁_eq_of_odd C, IH], split,
+    { simp[L₁_eq_of_odd C, IH], split,
       { rintros ⟨s, lt_s, s_even, rfl, pi⟩, refine ⟨s, nat.lt.step lt_s, s_even, rfl, pi⟩ },
       { rintros ⟨s, lt_s, s_even, rfl, pi⟩,
         have : s < t ∨ s = t, from lt_or_eq_of_le (nat.lt_succ_iff.mp lt_s),
@@ -130,37 +211,37 @@ begin
         { refine ⟨s, lt, s_even, rfl, pi⟩ }, { exfalso, simp[C] at s_even, contradiction } } } }
 end
 
-lemma mem_I₀_iff (t a : ℕ) :
-  a ∈ I₀ t ↔ ∃ s < t, (up[str] (Λ s)).length.bodd = tt ∧ a = (up[str] (Λ s)).weight ∧ directing_sentence₁ s :=
+lemma mem_L₀_iff (t a : ℕ) :
+  a ∈ L₀ t ↔ ∃ s < t, (up[str] (Λ s)).length.bodd = tt ∧ a = (up[str] (Λ s)).weight ∧ directing_sentence₁ s :=
 begin
   induction t with t IH,
   { simp },
   { rcases C : (up[str] (Λ t)).length.bodd with (C | C),
-    { simp[I₀_eq_of_even C, IH], split,
+    { simp[L₀_eq_of_even C, IH], split,
       { rintros ⟨s, lt_s, s_even, rfl, pi⟩, refine ⟨s, nat.lt.step lt_s, s_even, rfl, pi⟩ },
       { rintros ⟨s, lt_s, s_even, rfl, pi⟩,
         have : s < t ∨ s = t, from lt_or_eq_of_le (nat.lt_succ_iff.mp lt_s),
         rcases this with (lt | rfl),
         { refine ⟨s, lt, s_even, rfl, pi⟩ }, { exfalso, simp[C] at s_even, contradiction } } },
     { by_cases C₂ : directing_sentence₁ t,
-      { simp[I₀_eq_of_pi_of_odd C C₂, IH], split,
+      { simp[L₀_eq_of_pi_of_odd C C₂, IH], split,
         { rintros (rfl | ⟨s, lt, s_even, rfl, pi⟩),
           { exact ⟨t, lt_add_one t, C, rfl, C₂⟩ }, { refine ⟨s, nat.lt.step lt, s_even, rfl, pi⟩ } },
         { rintros ⟨s, lt_s, s_even, rfl, pi⟩,
           have : s < t ∨ s = t, from lt_or_eq_of_le (nat.lt_succ_iff.mp lt_s),
           rcases this with (lt | rfl), { right, refine ⟨s, lt, s_even, rfl, pi⟩ }, { left, simp } } },
-      { simp[I₀_eq_of_sigma_of_odd C C₂, IH], split,
+      { simp[L₀_eq_of_sigma_of_odd C C₂, IH], split,
         { rintros ⟨s, lt_s, s_even, rfl, pi⟩, refine ⟨s, nat.lt.step lt_s, s_even, rfl, pi⟩ },
         { rintros ⟨s, lt_s, s_even, rfl, pi⟩,
           have : s < t ∨ s = t, from lt_or_eq_of_le (nat.lt_succ_iff.mp lt_s),
           rcases this with (lt | rfl), { refine ⟨s, lt, s_even, rfl, pi⟩ }, { exfalso, contradiction } } } } }
 end
 
-lemma I₁_mono {s₁ s₂ : ℕ} (le : s₁ ≤ s₂) : I₁ s₁ ⊆ I₁ s₂ := λ a mem,
-by { simp [mem_I₁_iff] at mem ⊢, rcases mem with ⟨s, lt_s, h⟩, refine ⟨s, gt_of_ge_of_gt le lt_s, h⟩ }
+lemma L₁_mono {s₁ s₂ : ℕ} (le : s₁ ≤ s₂) : L₁ s₁ ⊆ L₁ s₂ := λ a mem,
+by { simp [mem_L₁_iff] at mem ⊢, rcases mem with ⟨s, lt_s, h⟩, refine ⟨s, gt_of_ge_of_gt le lt_s, h⟩ }
 
-lemma I₀_mono {s₁ s₂ : ℕ} (le : s₁ ≤ s₂) : I₀ s₁ ⊆ I₀ s₂ := λ a mem,
-by { simp [mem_I₀_iff] at mem ⊢, rcases mem with ⟨s, lt_s, h⟩, refine ⟨s, gt_of_ge_of_gt le lt_s, h⟩ }
+lemma L₀_mono {s₁ s₂ : ℕ} (le : s₁ ≤ s₂) : L₀ s₁ ⊆ L₀ s₂ := λ a mem,
+by { simp [mem_L₀_iff] at mem ⊢, rcases mem with ⟨s, lt_s, h⟩, refine ⟨s, gt_of_ge_of_gt le lt_s, h⟩ }
 
 @[simp] lemma pi_outcome_iff_of_even {s} (even : (up[str] (Λ s)).length.bodd = ff) :
   (Λ_thick.out s).is_pi ↔ directing_sentence₀ s :=
@@ -193,9 +274,9 @@ by { simp[←pi_outcome_iff_of_odd odd], cases Λ_thick.out s; simp[infinity, ze
 lemma sigma_preservation_of_pi_of_even
   {s₁ s₂} (even : (up[str] (Λ s₁)).length.bodd = ff) (pi : directing_sentence₀ s₁) 
   (on_truepath : up[str] (Λ s₁) ⊆' Λ[str] Λ) (le : s₁ ≤ s₂) {a : ℕ} (bound : a ≤ (λ[str] (Λ s₁)).weight) :
-  a ∈ I₀ s₂ → a ∈ I₀ s₁ :=
+  a ∈ L₀ s₂ → a ∈ L₀ s₁ :=
 begin
-  simp only [mem_I₀_iff],
+  simp only [mem_L₀_iff],
   rintros ⟨s, lt_s, odd, rfl, pi_s⟩,
   have : s < s₁ ∨ s = s₁ ∨ s₁ < s, exact trichotomous s s₁, rcases this with (lt_s | lt_s),
   { refine ⟨s, lt_s, odd, rfl, pi_s⟩ },
@@ -209,17 +290,17 @@ end
 lemma sigma_preservation_of_even_aux
   {η : Tree 1} {s₀} {lt : η ⊂ᵢ (Λ[str] Λ) s₀} (sigma : (out ⟨η, lt⟩).is_sigma) (even : η.length.bodd = ff) :
   ∃ s, directing_sentence₀ s ∧
-    up[str] (Λ s) = η ∧ ⟦η.length.div2⟧ᵪ^(chr I₀_inf) [(λ[str] (Λ s)).weight] η.weight = ff :=
+    up[str] (Λ s) = η ∧ ⟦η.length.div2⟧ᵪ^(chr I₀) [(λ[str] (Λ s)).weight] η.weight = ff :=
 begin
   rcases str.Lambda_sigma_outcome_of_thick Λ Λ_thick lt sigma with ⟨s, rfl, eq_out, pi⟩,
   have pi : directing_sentence₀ s, from (pi_outcome_iff_of_even even).mp pi,
-  have : ∀ a : ℕ, a < (λ[str] (Λ s)).weight → (I₀ s).chr a = chr I₀_inf a,
+  have : ∀ a : ℕ, a < (λ[str] (Λ s)).weight → (L₀ s).chr a = chr I₀ a,
   { intros a bound, simp[←bool.coe_bool_iff],
-    show a ∈ I₀ s ↔ I₀_inf a,
+    show a ∈ L₀ s ↔ I₀ a,
     refine ⟨λ h, ⟨s, h⟩, λ ⟨t, h⟩, sigma_preservation_of_pi_of_even
-      even pi ⟨s₀, lt.suffix⟩ (le_max_left s t) (le_of_lt bound) (I₀_mono (le_max_right s t) h)⟩ },
-  have : ⟦(up[str] (Λ s)).length.div2⟧ᵪ^(I₀ s).chr [(λ[str] (Λ s)).weight] =
-    ⟦(up[str] (Λ s)).length.div2⟧ᵪ^(chr I₀_inf) [(λ[str] (Λ s)).weight],
+      even pi ⟨s₀, lt.suffix⟩ (le_max_left s t) (le_of_lt bound) (L₀_mono (le_max_right s t) h)⟩ },
+  have : ⟦(up[str] (Λ s)).length.div2⟧ᵪ^(L₀ s).chr [(λ[str] (Λ s)).weight] =
+    ⟦(up[str] (Λ s)).length.div2⟧ᵪ^(chr I₀) [(λ[str] (Λ s)).weight],
     from rpartrec.univn_tot_use this,
   refine ⟨s, pi, rfl, _⟩,  
   simp[←this], exact pi
@@ -227,17 +308,17 @@ end
 
 lemma sigma_preservation_of_even
   {η : Tree 1} {s₀} {lt : η ⊂ᵢ (Λ[str] Λ) s₀} (sigma : (out ⟨η, lt⟩).is_sigma) (even : η.length.bodd = ff) :
-  η.weight ∈ I₁_inf ∧ ff ∈ ⟦η.length.div2⟧ᵪ^(chr I₀_inf) η.weight :=
+  η.weight ∈ I₁ ∧ ff ∈ ⟦η.length.div2⟧ᵪ^(chr I₀) η.weight :=
 by { rcases sigma_preservation_of_even_aux sigma even with ⟨s, pi, rfl, eqn⟩,
      simp[rpartrec.univn_complete],
-     refine ⟨mem_I₁_inf_of_pi_of_even even pi, (λ[str] (Λ s)).weight, eqn⟩}
+     refine ⟨mem_I₁_of_pi_of_even even pi, (λ[str] (Λ s)).weight, eqn⟩}
 
 lemma sigma_preservation_of_pi_of_odd
   {s₁ s₂} (odd : (up[str] (Λ s₁)).length.bodd = tt) (pi : directing_sentence₁ s₁) 
   (on_truepath : up[str] (Λ s₁) ⊆' Λ[str] Λ) (le : s₁ ≤ s₂) {a : ℕ} (bound : a ≤ (λ[str] (Λ s₁)).weight) :
-  a ∈ I₁ s₂ → a ∈ I₁ s₁:=
+  a ∈ L₁ s₂ → a ∈ L₁ s₁:=
 begin
-  simp only [mem_I₁_iff],
+  simp only [mem_L₁_iff],
   rintros ⟨s, lt_s, even, rfl, pi_s⟩,
   have : s < s₁ ∨ s = s₁ ∨ s₁ < s, exact trichotomous s s₁, rcases this with (lt_s | lt_s),
   { refine ⟨s, lt_s, even, rfl, pi_s⟩ },
@@ -251,17 +332,17 @@ end
 lemma sigma_preservation_of_odd_aux
   {η : Tree 1} {s₀} {lt : η ⊂ᵢ (Λ[str] Λ) s₀} (sigma : (out ⟨η, lt⟩).is_sigma) (odd : η.length.bodd = tt) :
   ∃ s, directing_sentence₁ s ∧
-    up[str] (Λ s) = η ∧ ⟦η.length.div2⟧ᵪ^(chr I₁_inf) [(λ[str] (Λ s)).weight] η.weight = ff :=
+    up[str] (Λ s) = η ∧ ⟦η.length.div2⟧ᵪ^(chr I₁) [(λ[str] (Λ s)).weight] η.weight = ff :=
 begin
   rcases str.Lambda_sigma_outcome_of_thick Λ Λ_thick lt sigma with ⟨s, rfl, eq_out, pi⟩,
   have pi : directing_sentence₁ s, from (pi_outcome_iff_of_odd odd).mp pi,
-  have : ∀ a : ℕ, a < (λ[str] (Λ s)).weight → (I₁ s).chr a = chr I₁_inf a,
+  have : ∀ a : ℕ, a < (λ[str] (Λ s)).weight → (L₁ s).chr a = chr I₁ a,
   { intros a bound, simp[←bool.coe_bool_iff],
-    show a ∈ I₁ s ↔ I₁_inf a,
+    show a ∈ L₁ s ↔ I₁ a,
     refine ⟨λ h, ⟨s, h⟩, λ ⟨t, h⟩, sigma_preservation_of_pi_of_odd
-      odd pi ⟨s₀, lt.suffix⟩ (le_max_left s t) (le_of_lt bound) (I₁_mono (le_max_right s t) h)⟩ },
-  have : ⟦(up[str] (Λ s)).length.div2⟧ᵪ^(I₁ s).chr [(λ[str] (Λ s)).weight] =
-    ⟦(up[str] (Λ s)).length.div2⟧ᵪ^(chr I₁_inf) [(λ[str] (Λ s)).weight],
+      odd pi ⟨s₀, lt.suffix⟩ (le_max_left s t) (le_of_lt bound) (L₁_mono (le_max_right s t) h)⟩ },
+  have : ⟦(up[str] (Λ s)).length.div2⟧ᵪ^(L₁ s).chr [(λ[str] (Λ s)).weight] =
+    ⟦(up[str] (Λ s)).length.div2⟧ᵪ^(chr I₁) [(λ[str] (Λ s)).weight],
     from rpartrec.univn_tot_use this,
   refine ⟨s, pi, rfl, _⟩,  
   simp[←this], exact pi
@@ -269,17 +350,17 @@ end
 
 lemma sigma_preservation_of_odd
   {η : Tree 1} {s₀} {lt : η ⊂ᵢ (Λ[str] Λ) s₀} (sigma : (out ⟨η, lt⟩).is_sigma) (odd : η.length.bodd = tt) :
-  η.weight ∈ I₀_inf ∧ ff ∈ ⟦η.length.div2⟧ᵪ^(chr I₁_inf) η.weight :=
+  η.weight ∈ I₀ ∧ ff ∈ ⟦η.length.div2⟧ᵪ^(chr I₁) η.weight :=
 by { rcases sigma_preservation_of_odd_aux sigma odd with ⟨s, pi, rfl, eqn⟩,
      simp[rpartrec.univn_complete],
-     refine ⟨mem_I₀_inf_of_pi_of_odd odd pi, (λ[str] (Λ s)).weight, eqn⟩ }
+     refine ⟨mem_I₀_of_pi_of_odd odd pi, (λ[str] (Λ s)).weight, eqn⟩ }
 
 lemma nonmem_of_even
   {η : Tree 1} {t} {lt : η ⊂ᵢ (Λ[str] Λ) t} (pi : (out ⟨η, lt⟩).is_pi) (even : η.length.bodd = ff) :
-  η.weight ∉ I₁_inf := λ mem,
+  η.weight ∉ I₁ := λ mem,
 begin
   rcases mem with ⟨s₀, mem⟩,
-  rcases (mem_I₁_iff s₀ η.weight).mp mem with ⟨s, lt_s, _, eq_weight, pi⟩,
+  rcases (mem_L₁_iff s₀ η.weight).mp mem with ⟨s, lt_s, _, eq_weight, pi⟩,
   have : η = up[str] (Λ s),
   { rcases str.le_Lambda_of_thick' Λ_thick ⟨t, lt.suffix⟩ with ⟨s₀, rfl, _⟩, simp at*,
     rcases str.eq_lambda_of_le_lambda' (str.up_le_lambda (Λ s)) with ⟨μ₀, le_μ₀, eq_up⟩,
@@ -292,10 +373,10 @@ end
 
 lemma nonmem_of_odd
   {η : Tree 1} {t} {lt : η ⊂ᵢ (Λ[str] Λ) t} (pi : (out ⟨η, lt⟩).is_pi) (odd : η.length.bodd = tt) :
-  η.weight ∉ I₀_inf := λ mem,
+  η.weight ∉ I₀ := λ mem,
 begin
   rcases mem with ⟨s₀, mem⟩,
-  rcases (mem_I₀_iff s₀ η.weight).mp mem with ⟨s, lt_s, _, eq_weight, pi⟩,
+  rcases (mem_L₀_iff s₀ η.weight).mp mem with ⟨s, lt_s, _, eq_weight, pi⟩,
   have : η = up[str] (Λ s),
   { rcases str.le_Lambda_of_thick' Λ_thick ⟨t, lt.suffix⟩ with ⟨s₀, rfl, _⟩, simp at*,
     rcases str.eq_lambda_of_le_lambda' (str.up_le_lambda (Λ s)) with ⟨μ₀, le_μ₀, eq_up⟩,
@@ -306,48 +387,48 @@ begin
   contradiction
 end
 
-lemma I₀_beq_exists(b : ℕ) :
-  ∃ s, ∀ a < b, a ∈ I₀ s ↔ a ∈ I₀_inf :=
+lemma L₀_beq_exists(b : ℕ) :
+  ∃ s, ∀ a < b, a ∈ L₀ s ↔ a ∈ I₀ :=
 begin
   induction b with b IH,
   { simp },
   { rcases IH with ⟨s₀, beq⟩,
-    by_cases C : b ∈ I₀_inf,
+    by_cases C : b ∈ I₀,
     { rcases C with ⟨s_b, mem⟩,
       refine ⟨max s₀ s_b, λ a bound, _⟩,
       split, { intros mem, refine ⟨_, mem⟩ },
       intros mem,
       have : a < b ∨ a = b, from lt_or_eq_of_le (nat.lt_succ_iff.mp bound),
       rcases this with (lt | rfl),
-      { have : a ∈ I₀ s₀, from (beq a lt).mpr mem, exact I₀_mono (le_max_left s₀ s_b) this },
-      { exact I₀_mono (le_max_right s₀ s_b) mem } },
+      { have : a ∈ L₀ s₀, from (beq a lt).mpr mem, exact L₀_mono (le_max_left s₀ s_b) this },
+      { exact L₀_mono (le_max_right s₀ s_b) mem } },
     { refine ⟨s₀, λ a bound, _⟩,
       have : a < b ∨ a = b, from lt_or_eq_of_le (nat.lt_succ_iff.mp bound),
       rcases this with (lt | rfl),
       { exact beq a lt },
-      { simp[C], intros mem, have : a ∈ I₀_inf, from ⟨s₀, mem⟩, contradiction } } }
+      { simp[C], intros mem, have : a ∈ I₀, from ⟨s₀, mem⟩, contradiction } } }
 end
 
-lemma I₁_beq_exists(b : ℕ) :
-  ∃ s, ∀ a < b, a ∈ I₁ s ↔ a ∈ I₁_inf :=
+lemma L₁_beq_exists(b : ℕ) :
+  ∃ s, ∀ a < b, a ∈ L₁ s ↔ a ∈ I₁ :=
 begin
   induction b with b IH,
   { simp },
   { rcases IH with ⟨s₀, beq⟩,
-    by_cases C : b ∈ I₁_inf,
+    by_cases C : b ∈ I₁,
     { rcases C with ⟨s_b, mem⟩,
       refine ⟨max s₀ s_b, λ a bound, _⟩,
       split, { intros mem, refine ⟨_, mem⟩ },
       intros mem,
       have : a < b ∨ a = b, from lt_or_eq_of_le (nat.lt_succ_iff.mp bound),
       rcases this with (lt | rfl),
-      { have : a ∈ I₁ s₀, from (beq a lt).mpr mem, exact I₁_mono (le_max_left s₀ s_b) this },
-      { exact I₁_mono (le_max_right s₀ s_b) mem } },
+      { have : a ∈ L₁ s₀, from (beq a lt).mpr mem, exact L₁_mono (le_max_left s₀ s_b) this },
+      { exact L₁_mono (le_max_right s₀ s_b) mem } },
     { refine ⟨s₀, λ a bound, _⟩,
       have : a < b ∨ a = b, from lt_or_eq_of_le (nat.lt_succ_iff.mp bound),
       rcases this with (lt | rfl),
       { exact beq a lt },
-      { simp[C], intros mem, have : a ∈ I₁_inf, from ⟨s₀, mem⟩, contradiction } } }
+      { simp[C], intros mem, have : a ∈ I₁, from ⟨s₀, mem⟩, contradiction } } }
 end
 
 lemma pi_substrategies_of_even_aux
@@ -362,26 +443,26 @@ end
 
 lemma pi_substrategies_of_even
   {η : Tree 1} {t} {lt : η ⊂ᵢ (Λ[str] Λ) t} (pi : (out ⟨η, lt⟩).is_pi) (even : η.length.bodd = ff) :
-  ¬ff ∈ ⟦η.length.div2⟧ᵪ^(chr I₀_inf) η.weight := λ A,
+  ¬ff ∈ ⟦η.length.div2⟧ᵪ^(chr I₀) η.weight := λ A,
 begin
-  have : ∃ s₀, ⟦η.length.div2⟧ᵪ^(chr I₀_inf) [s₀] η.weight = ff, from rpartrec.univn_complete.mp A,
+  have : ∃ s₀, ⟦η.length.div2⟧ᵪ^(chr I₀) [s₀] η.weight = ff, from rpartrec.univn_complete.mp A,
   rcases this with ⟨s₀, eq_ff⟩,
-  have : ∃ t, ∀ a < s₀, a ∈ I₀ t ↔ a ∈ I₀_inf, from I₀_beq_exists s₀,
+  have : ∃ t, ∀ a < s₀, a ∈ L₀ t ↔ a ∈ I₀, from L₀_beq_exists s₀,
   rcases this with ⟨t₀, beq⟩,
   have : ∃ s₁, s₀ < (λ[str] (Λ s₁)).weight, from str.lambda_infinitely Λ_thick (by simp) _,
   rcases this with ⟨s₁, lt_weight⟩,
   let s₂ := max t₀ s₁,
-  have : ∃ s > max t₀ s₁, ¬⟦(up[str] (Λ s)).length.div2⟧ᵪ^(I₀ s).chr [(λ[str] (Λ s)).weight] (up[str] (Λ s)).weight = ff ∧ 
+  have : ∃ s > max t₀ s₁, ¬⟦(up[str] (Λ s)).length.div2⟧ᵪ^(L₀ s).chr [(λ[str] (Λ s)).weight] (up[str] (Λ s)).weight = ff ∧ 
     up[str] (Λ s) = η, from pi_substrategies_of_even_aux pi even _,
   rcases this with ⟨s, lt_s, ne_ff, rfl⟩,
   have le_s₀ : s₀ ≤ (λ[str] (Λ s)).weight,
     calc s₀ ≤ (λ[str] (Λ s₁)).weight : le_of_lt lt_weight
         ... ≤ (λ[str] (Λ s)).weight : str.weight_lambda_le_mono (Λ_thick.le_mono_iff.mpr (le_of_lt (max_lt_iff.mp lt_s).2)),
-  have beq_s : ∀ a < s₀, (a ∈ I₀_inf ↔ a ∈ I₀ s),
+  have beq_s : ∀ a < s₀, (a ∈ I₀ ↔ a ∈ L₀ s),
   { intros a bound, split, 
-    { intros mem, have : a ∈ I₀ t₀, from (beq a bound).mpr mem, exact I₀_mono (le_of_lt (max_lt_iff.mp lt_s).1) this },
+    { intros mem, have : a ∈ L₀ t₀, from (beq a bound).mpr mem, exact L₀_mono (le_of_lt (max_lt_iff.mp lt_s).1) this },
     { intros mem, exact ⟨s, mem⟩ } },
-  have : ⟦(up[str] (Λ s)).length.div2⟧ᵪ^(I₀ s).chr [(λ[str] (Λ s)).weight] (up[str] (Λ s)).weight = ff,
+  have : ⟦(up[str] (Λ s)).length.div2⟧ᵪ^(L₀ s).chr [(λ[str] (Λ s)).weight] (up[str] (Λ s)).weight = ff,
     from rpartrec.univn_tot_mono_use (by { simp[←bool.coe_bool_iff], exact beq_s }) le_s₀ eq_ff,
   contradiction
 end
@@ -398,34 +479,34 @@ end
 
 lemma pi_substrategies_of_odd
   {η : Tree 1} {t} {lt : η ⊂ᵢ (Λ[str] Λ) t} (pi : (out ⟨η, lt⟩).is_pi) (odd : η.length.bodd = tt) :
-  ¬ff ∈ ⟦η.length.div2⟧ᵪ^(chr I₁_inf) η.weight := λ A,
+  ¬ff ∈ ⟦η.length.div2⟧ᵪ^(chr I₁) η.weight := λ A,
 begin
-  have : ∃ s₀, ⟦η.length.div2⟧ᵪ^(chr I₁_inf) [s₀] η.weight = ff, from rpartrec.univn_complete.mp A,
+  have : ∃ s₀, ⟦η.length.div2⟧ᵪ^(chr I₁) [s₀] η.weight = ff, from rpartrec.univn_complete.mp A,
   rcases this with ⟨s₀, eq_ff⟩,
-  have : ∃ t, ∀ a < s₀, a ∈ I₁ t ↔ a ∈ I₁_inf, from I₁_beq_exists s₀,
+  have : ∃ t, ∀ a < s₀, a ∈ L₁ t ↔ a ∈ I₁, from L₁_beq_exists s₀,
   rcases this with ⟨t₀, beq⟩,
   have : ∃ s₁, s₀ < (λ[str] (Λ s₁)).weight, from str.lambda_infinitely Λ_thick (by simp) _,
   rcases this with ⟨s₁, lt_weight⟩,
   let s₂ := max t₀ s₁,
-  have : ∃ s > max t₀ s₁, ¬⟦(up[str] (Λ s)).length.div2⟧ᵪ^(I₁ s).chr [(λ[str] (Λ s)).weight] (up[str] (Λ s)).weight = ff ∧ 
+  have : ∃ s > max t₀ s₁, ¬⟦(up[str] (Λ s)).length.div2⟧ᵪ^(L₁ s).chr [(λ[str] (Λ s)).weight] (up[str] (Λ s)).weight = ff ∧ 
     up[str] (Λ s) = η, from pi_substrategies_of_odd_aux pi odd _,
   rcases this with ⟨s, lt_s, ne_ff, rfl⟩,
   have le_s₀ : s₀ ≤ (λ[str] (Λ s)).weight,
     calc s₀ ≤ (λ[str] (Λ s₁)).weight : le_of_lt lt_weight
         ... ≤ (λ[str] (Λ s)).weight : str.weight_lambda_le_mono (Λ_thick.le_mono_iff.mpr (le_of_lt (max_lt_iff.mp lt_s).2)),
-  have beq_s : ∀ a < s₀, (a ∈ I₁_inf ↔ a ∈ I₁ s),
+  have beq_s : ∀ a < s₀, (a ∈ I₁ ↔ a ∈ L₁ s),
   { intros a bound, split, 
-    { intros mem, have : a ∈ I₁ t₀, from (beq a bound).mpr mem, exact I₁_mono (le_of_lt (max_lt_iff.mp lt_s).1) this },
+    { intros mem, have : a ∈ L₁ t₀, from (beq a bound).mpr mem, exact L₁_mono (le_of_lt (max_lt_iff.mp lt_s).1) this },
     { intros mem, exact ⟨s, mem⟩ } },
-  have : ⟦(up[str] (Λ s)).length.div2⟧ᵪ^(I₁ s).chr [(λ[str] (Λ s)).weight] (up[str] (Λ s)).weight = ff,
+  have : ⟦(up[str] (Λ s)).length.div2⟧ᵪ^(L₁ s).chr [(λ[str] (Λ s)).weight] (up[str] (Λ s)).weight = ff,
     from rpartrec.univn_tot_mono_use (by { simp[←bool.coe_bool_iff], exact beq_s }) le_s₀ eq_ff,
   contradiction
 end
 
 
-theorem not_I₁_le_I₀ : ¬I₁_inf ≤ₜ I₀_inf := λ hyp,
+theorem not_I₁_le_I₀ : ¬I₁ ≤ₜ I₀ := λ hyp,
 begin
-  have : ∃ e, ⟦e⟧ᵪ^(chr I₀_inf) = chr I₁_inf, from rpartrec.exists_index.mp (classical_iff.mp hyp),
+  have : ∃ e, ⟦e⟧ᵪ^(chr I₀) = chr I₁, from rpartrec.exists_index.mp (classical_iff.mp hyp),
   rcases this with ⟨e, lmm_e⟩,
   have : ∃ η, η ⊂' Λ[str] Λ ∧ η.length = bit0 e, from (str.Lambda_infinite Λ_thick).lt_length_eq (bit0 e),
   rcases this with ⟨η, ⟨s₀, lt⟩, eq_len⟩,
@@ -433,19 +514,19 @@ begin
   have eq_e : e = η.length.div2, { simp[eq_len] },  
   have : (out ⟨η, lt⟩).is_pi ∨ (out ⟨η, lt⟩).is_sigma, from pi_or_sigma (out ⟨η, lt⟩),
   rcases this with (pi | sigma),
-  { have : η.weight ∉ I₁_inf, from nonmem_of_even pi even,
-    have : ff ∈ ⟦e⟧ᵪ^(chr I₀_inf) η.weight, { simp[lmm_e], exact eq.symm ((chr_ff_iff _ _).mpr this) },
-    have : ff ∉ ⟦e⟧ᵪ^(chr I₀_inf) η.weight, rw eq_e, from pi_substrategies_of_even pi even,
+  { have : η.weight ∉ I₁, from nonmem_of_even pi even,
+    have : ff ∈ ⟦e⟧ᵪ^(chr I₀) η.weight, { simp[lmm_e], exact eq.symm ((chr_ff_iff _ _).mpr this) },
+    have : ff ∉ ⟦e⟧ᵪ^(chr I₀) η.weight, rw eq_e, from pi_substrategies_of_even pi even,
     contradiction },
-  { have : η.weight ∈ I₁_inf ∧ ff ∈ ⟦e⟧ᵪ^(chr I₀_inf) η.weight, rw eq_e, from sigma_preservation_of_even sigma even,
+  { have : η.weight ∈ I₁ ∧ ff ∈ ⟦e⟧ᵪ^(chr I₀) η.weight, rw eq_e, from sigma_preservation_of_even sigma even,
     rcases this with ⟨mem, nonmem⟩,
-    have : η.weight ∉ I₁_inf, { simp[lmm_e] at nonmem, exact (chr_ff_iff _ _).mp (eq.symm nonmem) },
+    have : η.weight ∉ I₁, { simp[lmm_e] at nonmem, exact (chr_ff_iff _ _).mp (eq.symm nonmem) },
     contradiction }
 end
 
-theorem not_I₀_le_I₁ : ¬I₀_inf ≤ₜ I₁_inf := λ hyp,
+theorem not_I₀_le_I₁ : ¬I₀ ≤ₜ I₁ := λ hyp,
 begin
-  have : ∃ e, ⟦e⟧ᵪ^(chr I₁_inf) = chr I₀_inf, from rpartrec.exists_index.mp (classical_iff.mp hyp),
+  have : ∃ e, ⟦e⟧ᵪ^(chr I₁) = chr I₀, from rpartrec.exists_index.mp (classical_iff.mp hyp),
   rcases this with ⟨e, lmm_e⟩,
   have : ∃ η, η ⊂' Λ[str] Λ ∧ η.length = bit1 e, from (str.Lambda_infinite Λ_thick).lt_length_eq (bit1 e),
   rcases this with ⟨η, ⟨s₀, lt⟩, eq_len⟩,
@@ -453,16 +534,17 @@ begin
   have eq_e : e = η.length.div2, { simp[eq_len] },  
   have : (out ⟨η, lt⟩).is_pi ∨ (out ⟨η, lt⟩).is_sigma, from pi_or_sigma (out ⟨η, lt⟩),
   rcases this with (pi | sigma),
-  { have : η.weight ∉ I₀_inf, from nonmem_of_odd pi odd,
-    have : ff ∈ ⟦e⟧ᵪ^(chr I₁_inf) η.weight, { simp[lmm_e], exact eq.symm ((chr_ff_iff _ _).mpr this) },
-    have : ff ∉ ⟦e⟧ᵪ^(chr I₁_inf) η.weight, rw eq_e, from pi_substrategies_of_odd pi odd,
+  { have : η.weight ∉ I₀, from nonmem_of_odd pi odd,
+    have : ff ∈ ⟦e⟧ᵪ^(chr I₁) η.weight, { simp[lmm_e], exact eq.symm ((chr_ff_iff _ _).mpr this) },
+    have : ff ∉ ⟦e⟧ᵪ^(chr I₁) η.weight, rw eq_e, from pi_substrategies_of_odd pi odd,
     contradiction },
-  { have : η.weight ∈ I₀_inf ∧ ff ∈ ⟦e⟧ᵪ^(chr I₁_inf) η.weight, rw eq_e, from sigma_preservation_of_odd sigma odd,
+  { have : η.weight ∈ I₀ ∧ ff ∈ ⟦e⟧ᵪ^(chr I₁) η.weight, rw eq_e, from sigma_preservation_of_odd sigma odd,
     rcases this with ⟨mem, nonmem⟩,
-    have : η.weight ∉ I₀_inf, { simp[lmm_e] at nonmem, exact (chr_ff_iff _ _).mp (eq.symm nonmem) },
+    have : η.weight ∉ I₀, { simp[lmm_e] at nonmem, exact (chr_ff_iff _ _).mp (eq.symm nonmem) },
     contradiction }
 end
 
-
+theorem incomparable_re_sets : ∃ I₀ I₁ : set ℕ, r.e. I₀ ∧ r.e. I₁ ∧ ¬I₁ ≤ₜ I₀ ∧ ¬I₀ ≤ₜ I₁ :=
+⟨I₀, I₁, I₀_re, I₁_re, not_I₁_le_I₀, not_I₀_le_I₁⟩
 
 end friedberg_muchnik
